saturation framework: minor clean ups

Saturation_Framework/Labeled_Lifting_to_Non_Ground_Calculi.thy
@@ -6,7 +6,8 @@ theory Labeled_Lifting_to_Non_Ground_Calculi
   imports Lifting_to_Non_Ground_Calculi
 begin
 
-locale labeled_lifting_w_wf_ord_family = lifting_with_wf_ordering_family Bot_F Inf_F Bot_G entails_G Inf_G Red_Inf_G Red_F_G \<G>_F \<G>_Inf Prec_F
+locale labeled_lifting_w_wf_ord_family =
+  lifting_with_wf_ordering_family Bot_F Inf_F Bot_G entails_G Inf_G Red_Inf_G Red_F_G \<G>_F \<G>_Inf Prec_F
   for
     Bot_F :: "'f set" and
     Inf_F :: "'f inference set" and
@@ -22,7 +23,8 @@ locale labeled_lifting_w_wf_ord_family = lifting_with_wf_ordering_family Bot_F I
     l :: \<open>'l itself\<close> and
     Inf_FL :: \<open>('f \<times> 'l) inference set\<close>
   assumes
-    Inf_F_to_Inf_FL: \<open>\<iota>\<^sub>F \<in> Inf_F \<Longrightarrow> length (Ll :: 'l list) = length (prems_of \<iota>\<^sub>F) \<Longrightarrow> \<exists>L0. Infer (zip (prems_of \<iota>\<^sub>F) Ll) (concl_of \<iota>\<^sub>F, L0) \<in> Inf_FL\<close> and
+    Inf_F_to_Inf_FL: \<open>\<iota>\<^sub>F \<in> Inf_F \<Longrightarrow> length (Ll :: 'l list) = length (prems_of \<iota>\<^sub>F) \<Longrightarrow>
+      \<exists>L0. Infer (zip (prems_of \<iota>\<^sub>F) Ll) (concl_of \<iota>\<^sub>F, L0) \<in> Inf_FL\<close> and
     Inf_FL_to_Inf_F: \<open>\<iota>\<^sub>F\<^sub>L \<in> Inf_FL \<Longrightarrow> Infer (map fst (prems_of \<iota>\<^sub>F\<^sub>L)) (fst (concl_of \<iota>\<^sub>F\<^sub>L)) \<in> Inf_F\<close>
 begin
 
@@ -59,7 +61,8 @@ next
 next
   fix CL
   show "\<G>_F_L CL \<inter> Bot_G \<noteq> {} \<longrightarrow> CL \<in> Bot_FL"
-    unfolding \<G>_F_L_def Bot_FL_def using Bot_cond by (metis SigmaE UNIV_I UNIV_Times_UNIV mem_Sigma_iff prod.sel(1))
+    unfolding \<G>_F_L_def Bot_FL_def using Bot_cond
+    by (metis SigmaE UNIV_I UNIV_Times_UNIV mem_Sigma_iff prod.sel(1))
 next
   fix \<iota>
   assume \<open>\<iota> \<in> Inf_FL\<close>
@@ -70,10 +73,14 @@ qed
 definition Labeled_Empty_Order :: \<open> ('f \<times> 'l) \<Rightarrow> ('f \<times> 'l) \<Rightarrow> bool\<close> where
   "Labeled_Empty_Order C1 C2 \<equiv> False" 
 
-sublocale labeled_lifting_w_empty_ord_family : lifting_with_wf_ordering_family Bot_FL Inf_FL Bot_G entails_G Inf_G Red_Inf_G Red_F_G \<G>_F_L \<G>_Inf_L "\<lambda>g. Labeled_Empty_Order" 
+sublocale labeled_lifting_w_empty_ord_family :
+  lifting_with_wf_ordering_family Bot_FL Inf_FL Bot_G entails_G Inf_G Red_Inf_G Red_F_G
+    \<G>_F_L \<G>_Inf_L "\<lambda>g. Labeled_Empty_Order" 
 proof
-  show "po_on Labeled_Empty_Order UNIV" unfolding Labeled_Empty_Order_def po_on_def by (simp add: transp_onI wfp_on_imp_irreflp_on)
-  show "wfp_on Labeled_Empty_Order UNIV" unfolding wfp_on_def Labeled_Empty_Order_def by simp
+  show "po_on Labeled_Empty_Order UNIV"
+    unfolding Labeled_Empty_Order_def po_on_def by (simp add: transp_onI wfp_on_imp_irreflp_on)
+  show "wfp_on Labeled_Empty_Order UNIV"
+    unfolding wfp_on_def Labeled_Empty_Order_def by simp
 qed
 
 notation "labeled_standard_lifting.entails_\<G>" (infix "\<Turnstile>\<G>L" 50)
@@ -119,11 +126,18 @@ proof clarify
 qed
 
 text "lemma:labeled-static-ref-compl"
-lemma "static_refutational_complete_calculus Bot_F Inf_F (\<Turnstile>\<G>) Red_Inf_\<G> Red_F_\<G> \<Longrightarrow> static_refutational_complete_calculus Bot_FL Inf_FL (\<Turnstile>\<G>L) labeled_lifting_w_empty_ord_family.Red_Inf_\<G> labeled_lifting_w_empty_ord_family.Red_F_\<G>"
+lemma "static_refutational_complete_calculus Bot_F Inf_F (\<Turnstile>\<G>) Red_Inf_\<G> Red_F_\<G> \<Longrightarrow>
+  static_refutational_complete_calculus Bot_FL Inf_FL (\<Turnstile>\<G>L)
+    labeled_lifting_w_empty_ord_family.Red_Inf_\<G> labeled_lifting_w_empty_ord_family.Red_F_\<G>"
   unfolding static_refutational_complete_calculus_def
 proof (rule conjI impI; clarify)
-  interpret calculus_with_red_crit Bot_FL Inf_FL labeled_standard_lifting.entails_\<G> labeled_lifting_w_empty_ord_family.Red_Inf_\<G> labeled_lifting_w_empty_ord_family.Red_F_\<G> by (simp add: labeled_lifting_w_empty_ord_family.lifted_calculus_with_red_crit.calculus_with_red_crit_axioms)
-  show "calculus_with_red_crit Bot_FL Inf_FL (\<Turnstile>\<G>L) labeled_lifting_w_empty_ord_family.Red_Inf_\<G> labeled_lifting_w_empty_ord_family.Red_F_\<G>" by standard
+  interpret calculus_with_red_crit Bot_FL Inf_FL labeled_standard_lifting.entails_\<G>
+    labeled_lifting_w_empty_ord_family.Red_Inf_\<G> labeled_lifting_w_empty_ord_family.Red_F_\<G>
+    by (simp add:
+      labeled_lifting_w_empty_ord_family.lifted_calculus_with_red_crit.calculus_with_red_crit_axioms)
+  show "calculus_with_red_crit Bot_FL Inf_FL (\<Turnstile>\<G>L) labeled_lifting_w_empty_ord_family.Red_Inf_\<G>
+    labeled_lifting_w_empty_ord_family.Red_F_\<G>"
+    by standard
 next
   assume
     calc: "calculus_with_red_crit Bot_F Inf_F (\<Turnstile>\<G>) Red_Inf_\<G> Red_F_\<G>" and
@@ -145,7 +159,8 @@ next
     define N where "N = fst ` Nl"
     have N_sat: "empty_order_lifting.lifted_calculus_with_red_crit.saturated N"
       using N_def Nl_sat labeled_saturation_lifting by blast 
-    have N_entails_B: "N \<Turnstile>\<G> {B}" using Nl_entails_Bl unfolding labeled_entailment_lifting N_def B_def by force
+    have N_entails_B: "N \<Turnstile>\<G> {B}"
+      using Nl_entails_Bl unfolding labeled_entailment_lifting N_def B_def by force
     have "\<exists>B' \<in> Bot_F. B' \<in> N" using B_in N_sat N_entails_B static_axioms[of B N] by blast
     then obtain B' where in_Bot: "B' \<in> Bot_F" and in_N: "B' \<in> N" by force
     then have "B' \<in> fst ` Bot_FL" unfolding Bot_FL_def by fastforce
@@ -158,7 +173,8 @@ qed
 
 end
 
-locale labeled_lifting_with_red_crit_family = no_labels: standard_lifting_with_red_crit_family Inf_F Bot_G Inf_G Q entails_q Red_Inf_q Red_F_q Bot_F \<G>_F_q \<G>_Inf_q "\<lambda>g. Empty_Order"
+locale labeled_lifting_with_red_crit_family = no_labels: standard_lifting_with_red_crit_family Inf_F
+  Bot_G Inf_G Q entails_q Red_Inf_q Red_F_q Bot_F \<G>_F_q \<G>_Inf_q "\<lambda>g. Empty_Order"
   for
     Bot_F :: "'f set" and
     Inf_F :: "'f inference set" and
@@ -201,7 +217,8 @@ definition Labeled_Empty_Order :: \<open> ('f \<times> 'l) \<Rightarrow> ('f \<t
   "Labeled_Empty_Order C1 C2 \<equiv> False" 
 
 definition Red_F_\<G>_empty_L_q :: "'q \<Rightarrow> ('f \<times> 'l) set \<Rightarrow> ('f \<times> 'l) set" where
-  "Red_F_\<G>_empty_L_q q N = {C. \<forall>D \<in> \<G>_F_L_q q C. D \<in> Red_F_q q (\<G>_set_L_q q N) \<or> (\<exists>E \<in> N. Labeled_Empty_Order E C \<and> D \<in> \<G>_F_L_q q E)}"
+  "Red_F_\<G>_empty_L_q q N = {C. \<forall>D \<in> \<G>_F_L_q q C. D \<in> Red_F_q q (\<G>_set_L_q q N) \<or>
+    (\<exists>E \<in> N. Labeled_Empty_Order E C \<and> D \<in> \<G>_F_L_q q E)}"
 
 definition Red_F_\<G>_empty_L :: "('f \<times> 'l) set \<Rightarrow> ('f \<times> 'l) set" where
   "Red_F_\<G>_empty_L N = \<Inter> {X N |X. X \<in> (Red_F_\<G>_empty_L_q ` UNIV)}"
@@ -212,7 +229,8 @@ definition entails_\<G>_L_q :: "'q \<Rightarrow> ('f \<times> 'l) set \<Rightarr
 definition entails_\<G>_L_Q :: "('f \<times> 'l) set \<Rightarrow> ('f \<times> 'l) set \<Rightarrow> bool" (infix "\<Turnstile>\<inter>L" 50) where
   "entails_\<G>_L_Q N1 N2 \<equiv> \<forall>q. entails_\<G>_L_q q N1 N2"
 
-lemma lifting_q: "labeled_lifting_w_wf_ord_family Bot_F Inf_F Bot_G (entails_q q) Inf_G (Red_Inf_q q) (Red_F_q q) (\<G>_F_q q) (\<G>_Inf_q q) (\<lambda>g. Empty_Order) Inf_FL"
+lemma lifting_q: "labeled_lifting_w_wf_ord_family Bot_F Inf_F Bot_G (entails_q q) Inf_G (Red_Inf_q q)
+  (Red_F_q q) (\<G>_F_q q) (\<G>_Inf_q q) (\<lambda>g. Empty_Order) Inf_FL"
 proof -
   fix q
   show "labeled_lifting_w_wf_ord_family Bot_F Inf_F Bot_G (entails_q q) Inf_G (Red_Inf_q q)
@@ -255,7 +273,8 @@ proof -
     by (simp add: lifting_with_wf_ordering_family_axioms.intro lifting_with_wf_ordering_family_def)
 qed
 
-lemma all_lifted_red_crit: "calculus_with_red_crit Bot_FL Inf_FL (entails_\<G>_L_q q) (Red_Inf_\<G>_L_q q) (Red_F_\<G>_empty_L_q q)"
+lemma all_lifted_red_crit: "calculus_with_red_crit Bot_FL Inf_FL (entails_\<G>_L_q q) (Red_Inf_\<G>_L_q q)
+  (Red_F_\<G>_empty_L_q q)"
 proof -
   fix q
   interpret ord_q_lifting: lifting_with_wf_ordering_family Bot_FL Inf_FL Bot_G "entails_q q" Inf_G
@@ -267,14 +286,16 @@ proof -
     unfolding Red_Inf_\<G>_L_q_def ord_q_lifting.Red_Inf_\<G>_def \<G>_set_L_q_def by simp
   moreover have "Red_F_\<G>_empty_L_q q = ord_q_lifting.Red_F_\<G>"
     unfolding Red_F_\<G>_empty_L_q_def ord_q_lifting.Red_F_\<G>_def \<G>_set_L_q_def by simp
-  ultimately show "calculus_with_red_crit Bot_FL Inf_FL (entails_\<G>_L_q q) (Red_Inf_\<G>_L_q q) (Red_F_\<G>_empty_L_q q)"
+  ultimately show "calculus_with_red_crit Bot_FL Inf_FL (entails_\<G>_L_q q) (Red_Inf_\<G>_L_q q)
+    (Red_F_\<G>_empty_L_q q)"
     using ord_q_lifting.lifted_calculus_with_red_crit.calculus_with_red_crit_axioms by argo
 qed
 
 lemma all_lifted_cons_rel: "consequence_relation Bot_FL (entails_\<G>_L_q q)"
 proof -
   fix q
-  interpret q_red_crit: calculus_with_red_crit Bot_FL Inf_FL "entails_\<G>_L_q q" "Red_Inf_\<G>_L_q q" "Red_F_\<G>_empty_L_q q"
+  interpret q_red_crit: calculus_with_red_crit Bot_FL Inf_FL "entails_\<G>_L_q q" "Red_Inf_\<G>_L_q q"
+    "Red_F_\<G>_empty_L_q q"
     using all_lifted_red_crit .
   show "consequence_relation Bot_FL (entails_\<G>_L_q q)"
     using q_red_crit.consequence_relation_axioms . 
@@ -285,7 +306,8 @@ sublocale labeled_cons_rel_family: consequence_relation_family Bot_FL Q entails_
   unfolding Bot_FL_def
   by (simp add: consequence_relation_family.intro)
 
-sublocale with_labels: calculus_with_red_crit_family Bot_FL Inf_FL Q entails_\<G>_L_q Red_Inf_\<G>_L_q Red_F_\<G>_empty_L_q
+sublocale with_labels: calculus_with_red_crit_family Bot_FL Inf_FL Q entails_\<G>_L_q Red_Inf_\<G>_L_q
+  Red_F_\<G>_empty_L_q
   using calculus_with_red_crit_family.intro[OF labeled_cons_rel_family.consequence_relation_family_axioms]
     all_lifted_cons_rel
   by (simp add: all_lifted_red_crit calculus_with_red_crit_family_axioms_def) 
@@ -310,7 +332,8 @@ proof clarify
   have i_in_q: "\<iota> \<in> Red_Inf_\<G>_L_q q NL" using i_in_inter image_eqI by blast
   then have i_in: "\<iota> \<in> Inf_FL" unfolding Red_Inf_\<G>_L_q_def by blast
   have to_F_in: "to_F \<iota> \<in> Inf_F" unfolding to_F_def using Inf_FL_to_Inf_F[OF i_in] .
-  have subs_red: "\<G>_Inf_L_q q \<iota> \<subseteq> Red_Inf_q q (\<G>_set_L_q q NL)" using i_in_q unfolding Red_Inf_\<G>_L_q_def by blast
+  have subs_red: "\<G>_Inf_L_q q \<iota> \<subseteq> Red_Inf_q q (\<G>_set_L_q q NL)"
+    using i_in_q unfolding Red_Inf_\<G>_L_q_def by blast
   then have "\<G>_Inf_q q (to_F \<iota>) \<subseteq> Red_Inf_q q (no_labels.\<G>_set_q q (fst ` NL))"
     unfolding \<G>_Inf_L_q_def \<G>_set_L_q_def no_labels.\<G>_set_q_def \<G>_F_L_q_def by simp
   then show "to_F \<iota> \<in> no_labels.Red_Inf_\<G>_q q (fst ` NL)"
@@ -372,15 +395,17 @@ next
       Bl_in: \<open>Bl \<in> Bot_FL\<close> and
       Nl_sat: \<open>with_labels.inter_red_crit_calculus.saturated Nl\<close> and
       Nl_entails_Bl: \<open>Nl \<Turnstile>\<inter>L {Bl}\<close>
-    have static_axioms: "B \<in> Bot_F \<longrightarrow> no_labels.lifted_calc_w_red_crit_family.inter_red_crit_calculus.saturated N
-      \<longrightarrow> N \<Turnstile>\<inter> {B} \<longrightarrow> (\<exists>B'\<in>Bot_F. B' \<in> N)" for B N
+    have static_axioms: "B \<in> Bot_F \<longrightarrow>
+      no_labels.lifted_calc_w_red_crit_family.inter_red_crit_calculus.saturated N \<longrightarrow>
+      N \<Turnstile>\<inter> {B} \<longrightarrow> (\<exists>B'\<in>Bot_F. B' \<in> N)" for B N
       using static[unfolded static_refutational_complete_calculus_axioms_def] by fast
     define B where "B = fst Bl"
     have B_in: "B \<in> Bot_F" using Bl_in Bot_FL_def B_def SigmaE by force
     define N where "N = fst ` Nl"
     have N_sat: "no_labels.lifted_calc_w_red_crit_family.inter_red_crit_calculus.saturated N"
       using N_def Nl_sat labeled_family_saturation_lifting by blast
-    have N_entails_B: "N \<Turnstile>\<inter> {B}" using Nl_entails_Bl unfolding labeled_entailment_lifting N_def B_def by force
+    have N_entails_B: "N \<Turnstile>\<inter> {B}"
+      using Nl_entails_Bl unfolding labeled_entailment_lifting N_def B_def by force
     have "\<exists>B' \<in> Bot_F. B' \<in> N" using B_in N_sat N_entails_B static_axioms[of B N] by blast
     then obtain B' where in_Bot: "B' \<in> Bot_F" and in_N: "B' \<in> N" by force
     then have "B' \<in> fst ` Bot_FL" unfolding Bot_FL_def by fastforce
